theories/TM/Code/BinNumbers/EncodeBinNumbers.v
@@ -1,9 +1,8 @@
 (** * Encoding for binary numbers *)
 
 From Undecidability Require Import TM.Prelim Code.
-From Undecidability Require Import ArithPrelim.
-From PslBase Require Export Bijection.
-Require Export BinNums. (* Warning: There also is a constructor called [N] for the type [move] *)
+From PslBase Require Import Bijection.
+From Coq Require Export BinNums. (* Warning: There also is a constructor called [N] for the type [move] *)
 
 
 (* We use Coq's standard types [positive] and [N] *)
