theories/TM/Hoare/HoareNth.v
@@ -1,0 +1,128 @@
+(* ** Verification of [Nth] with the Hoare framework *)
+
+From Undecidability Require Import ProgrammingTools.
+From Undecidability Require Import Hoare.Hoare.
+From Undecidability Require Import CaseNat CaseList.
+From Undecidability Require Import ListTM.
+
+Arguments plus : simpl never.
+Arguments mult : simpl never.
+
+
+Section Nth.
+
+  Variable (sig sigX : finType) (X : Type) (cX : codable sigX X).
+  Variable (retr1 : Retract (sigList sigX) sig) (retr2 : Retract sigNat sig).
+  Local Existing Instance retr_X_list'.
+
+  Definition Nth'_Step_steps_CaseList (xs : list X) :=
+    match xs with
+    | x :: xs' => 1 + CaseList_steps_cons x + Reset_steps x
+    | nil => 1 + CaseList_steps_nil
+    end.
+
+  Definition Nth'_Step_steps' (xs : list X) (n : nat) :=
+    match n with
+    | S n' => 1 + CaseNat_steps + Nth'_Step_steps_CaseList xs
+    | O' => 1 + CaseNat_steps + CaseList_steps xs
+    end.
+
+  Lemma Nth'_Step_SpecT_size (n : nat) (xs : list X) (ss : Vector.t nat 3) :
+    TripleT
+      (tspec (withSpace (SpecVector [|Contains _ xs; Contains _ n; Void|]) ss))
+      (Nth'_Step_steps xs n) (Nth'_Step retr1 retr2)
+      (fun yout =>
+         tspec (withSpace
+                  match yout, n, xs with
+                  | None,       S n', x::xs' => SpecVector [|Contains _ xs'; Contains _ n'; Void|]
+                  | Some true,     0, x::xs' => SpecVector [|Contains _ xs'; Contains _ 0;  Contains _ x|]
+                  | Some false,    O,   nil => SpecVector [|Contains _ nil; Contains _ 0;  Void|]
+                  | Some false, S n',   nil => SpecVector [|Contains _ nil; Contains _ n'; Void|]
+                  | _, _, _ => SpecFalse
+                  end (appSize (Nth'_Step_size n xs) ss))).
+  Proof.
+    unfold Nth'_Step.
+    eapply If_SpecT with (k1 := CaseNat_steps) (k2 := Nth'_Step_steps_CaseList xs) (k3 := CaseList_steps xs).
+    - hstep; cbn.
+      hstep; cbn. (* or [eapply ChangeAlphabet_SpecT_space_pre.] *)
+      hstep; cbn. cbn. tspec_ext.
+    - cbn. destruct n as [ | n']; cbn in *; auto.
+      (** Like in the Realisation proof, we make a case-distinction over the value of [xs]. *)
+      destruct xs as [ | x xs']; cbn in *; auto.
+      + eapply If_SpecT with (k2 := 0).
+        * hstep; cbn. hstep; cbn. hstep; cbn. cbn. tspec_ext.
+        * cbn. auto. (* The "Then" case of the "If CaseList". We are not in this state, since [xs=nil]. *)
+        * cbn. hstep; cbn. hstep; cbn. cbn. intros _. tspec_ext.
+        * cbn. intros tin yout tout. destruct yout; cbn in *; auto.
+      + eapply If_SpecT.
+        * hstep; cbn. hstep; cbn. hstep; cbn. cbn. tspec_ext.
+        * cbn. hstep; cbn. hstep; cbn. apply Reset_SpecT_space. cbn. intros _. tspec_ext.
+        * cbn. auto. (* The "Else" case of the "If CaseList". We are not in this state, since [xs=x::xs']. *)
+        * cbn. intros tin yout tout. destruct yout; cbn in *; auto.
+    - cbn. destruct n as [ | n']; cbn in *; auto.
+      hstep; cbn. hstep; cbn. hstep; cbn. hstep; cbn.
+      cbn. tspec_ext.
+      intros yout tout. destruct yout, xs as [ | x xs']; cbn in *; auto.
+      + intros. tspec_ext.
+      + intros. tspec_ext.
+    - intros ? ? ? ? ?. destruct yout, n as [ | n'], xs as [ | x xs']; cbn in *; auto.
+  Qed.
+
+  Lemma Nth'_Loop_SpecT_size xs n (ss : Vector.t nat 3) :
+    TripleT
+      (tspec (withSpace (SpecVector [|Contains _ xs; Contains _ n; Void|]) ss))
+      (Nth'_Loop_steps xs n) (Nth'_Loop retr1 retr2)
+      (fun yout =>
+         tspec
+           (withSpace
+              match yout, nth_error xs n with
+              | true, Some x => SpecVector [|Contains _ (skipn (S n) xs); Contains _ (n - (S (length xs))); Contains _ x|]
+              | false, None  => SpecVector [|Contains _ (skipn (S n) xs); Contains _ (n - (S (length xs))); Void|]
+              | _, _ => SpecFalse
+              end
+              (appSize (Nth'_Loop_size n xs) ss))).
+  Proof.
+    eapply While_SpecT with (P := fun '(xs,n,ss) => _) (Q := fun '(xs,n,ss) => _) (R := fun '(xs,n,ss) => _) (g := fun '(xs,n,ss) => _) (f := fun '(xs,n,ss) => _) (x := (xs,n,ss));
+      clear xs n ss; intros ((xs,n),ss).
+    - apply Nth'_Step_SpecT_size.
+    - cbn. intros yout tmid tout H1 H2.
+      destruct yout, n as [ | n'], xs as [ | x xs']; cbn in *; auto.
+      replace (n' - 0) with n' by omega. auto.
+    - cbn. intros yout tmid tout H1.
+      destruct n as [ | n'], xs as [ | x xs']; cbn in *; auto.
+      eexists (xs', n', _). repeat split; cbn.
+      + eauto.
+      + reflexivity.
+      + eauto.
+  Qed.
+
+  Lemma Nth'_SpecT_size (xs : list X) (n : nat) (ss : Vector.t nat 4) :
+    TripleT
+      (tspec (withSpace (SpecVector [|Contains _ xs; Contains _ n; Void; Void|]) ss))
+      (Nth'_steps xs n) (Nth' retr1 retr2)
+      (fun yout =>
+         tspec (withSpace
+                  match yout, nth_error xs n with
+                  | true, Some x => SpecVector [|Contains _ xs; Void; Contains _ x; Void|]
+                  | false, None => SpecVector [|Contains _ xs; Void; Void; Void|]
+                  | _, _ => SpecFalse
+                  end (appSize (Nth'_size xs n) ss))).
+  Proof.
+    unfold Nth'.
+    hstep; cbn. hstep; cbn. apply CopyValue_SpecT_size.
+    cbn. intros _. eapply If_SpecT; cbn.
+    - hstep; cbn. eapply ConsequenceT_pre. apply Nth'_Loop_SpecT_size. tspec_ext. reflexivity.
+    - cbn. destruct (nth_error xs n) as [ x | ]; cbn in *; auto.
+      hstep; cbn. hstep; cbn. hstep; cbn. apply Reset_SpecT_space with (X := list X).
+      cbn. intros []. eauto. hstep; cbn. apply Reset_SpecT_space with (X := nat). reflexivity.
+      cbn. intros _. auto.
+    - cbn. destruct (nth_error xs n) as [ x | ]; cbn in *; auto.
+      hstep; cbn. hstep; cbn. hstep; cbn. apply Reset_SpecT_space with (X := list X).
+      cbn. intros []. eauto. hstep; cbn. apply Reset_SpecT_space with (X := nat). reflexivity.
+      cbn. intros _. auto.
+    - cbn. intros tin yout tout ? ?. cbn. destruct yout; cbn in *; auto.
+    - unfold Nth'_steps. cbn. omega.
+  Qed.
+
+
+End Nth.
